Tealeaves/Backends/DB/DB.v
@@ -5,16 +5,14 @@ From Tealeaves.Theory Require Import
   DecoratedTraversableFunctor
   DecoratedTraversableMonad.
 
-
 From Tealeaves Require Import
   Backends.LN.
 From Tealeaves.Adapters Require Import
   MonadToApplicative
   KleisliToCategorical.Monad.
 
-Open Scope nat_scope.
-
 Import PeanoNat.Nat.
+Import Coq.Init.Nat. (* Nat notations *)
 
 Import
   Product.Notations
@@ -29,11 +27,30 @@ Import
   DecoratedContainerFunctor.Notations
   DecoratedTraversableMonad.Notations.
 
-Import Coq.Init.Nat. (* Nat notations *)
-
 #[local] Generalizable Variables W T U.
 
 Open Scope nat_scope.
+
+(* Iterate an endofunction <<n>> times *)
+Fixpoint iterate (n : nat) {A : Type} (f : A -> A) :=
+  match n with
+  | 0 => @id A
+  | S n' => iterate n' f ∘ f
+  end.
+
+Lemma iterate_rw0 : forall {A : Type} (f : A -> A),
+    iterate 0 f = id.
+Proof.
+  reflexivity.
+Qed.
+
+Lemma iterate_rw1 : forall (n : nat) {A : Type} (f : A -> A),
+    iterate (S n) f = (iterate n f) ∘ f.
+Proof.
+  intros.
+  cbn.
+  reflexivity.
+Qed.
 
 (** ** De Bruijn operations as defined by Tealeaves *)
 (******************************************************************************)
@@ -42,6 +59,7 @@ Section ops.
   Context
     `{ret_inst : Return T}
       `{Mapd_T_inst : Mapd nat T}
+      `{Mapd_U_inst : Mapd nat U}
       `{Bindd_U_inst : Bindd nat T U}.
 
   Definition bound_in: nat -> nat -> bool :=
@@ -49,6 +67,7 @@ Section ops.
 
   (* Local function for incrementing free variables
      by <<n>> *)
+  (* n: A value by which to increment free indices *)
   Definition lift (n : nat) (p : nat * nat) : nat :=
     match p with
     | (depth, ix) =>
@@ -66,14 +85,35 @@ Section ops.
        adjusted to account for bound variables in scope
    *)
   (* TODO: Decrement free variables if necessary *)
-  Definition scoot : nat -> (nat -> T nat) -> (nat -> T nat)  :=
+  Definition scoot : nat -> (nat -> T nat) -> (nat -> T nat) :=
     fun depth σ ix =>
       if bound_in ix depth
       then ret ix
       else mapd (lift depth) (σ (ix - depth)).
 
+  Definition scoot_ren : nat -> (nat -> nat) -> (nat -> nat) :=
+    fun depth ρ ix =>
+      if bound_in ix depth
+      then ix
+      else
+        lift depth (0, ρ (ix - depth))
+             (* = ρ (ix - depth) + depth *).
+
+  Definition rename_loc (ρ : nat -> nat) (p: nat * nat): nat :=
+    match p with
+    | (depth, ix) => scoot_ren depth ρ ix
+    end.
+
+  Definition open_loc (σ : nat -> T nat) (p: nat * nat): T nat :=
+    match p with
+    | (depth, ix) => scoot depth σ ix
+    end.
+
+  Definition rename (ρ : nat -> nat) : U nat -> U nat :=
+    mapd (T := U) (rename_loc ρ).
+
   Definition open (σ : nat -> T nat) : U nat -> U nat :=
-    bindd (fun '(depth, ix) => scoot depth σ ix).
+    bindd (open_loc σ).
 
   Definition one (u: T nat): nat -> T nat :=
     fun n => if n =? 0 then u else ret n.
@@ -82,6 +122,142 @@ Section ops.
     open (one u).
 
 End ops.
+
+Implicit Types (ρ: nat -> nat).
+
+Section theory.
+
+  Lemma bound_in_zero: forall ix,
+      bound_in ix 0 = false.
+  Proof.
+    reflexivity.
+  Qed.
+
+  Lemma bound_in_lt: forall ix n,
+      ix < n ->
+      bound_in ix n = true.
+  Proof.
+    introv Hlt.
+    rewrite <- ltb_lt in Hlt.
+    destruct n; cbn in *; auto.
+  Qed.
+
+  Lemma bound_in_lt_iff: forall ix n,
+      ix < n <->
+      bound_in ix n = true.
+  Proof.
+    intros. split.
+    - apply bound_in_lt.
+    - cbn. destruct n.
+      + inversion 1.
+      + cbn.
+        rewrite OrdersEx.Nat_as_OT.leb_le.
+        lia.
+  Qed.
+
+  Lemma bound_in_ge: forall ix n,
+      ix >= n ->
+      bound_in ix n = false.
+  Proof.
+    introv Hlt.
+    destruct n; cbn; auto.
+    now rewrite leb_gt.
+  Qed.
+
+  Lemma bound_in_ge_iff: forall ix n,
+      ix >= n <->
+      bound_in ix n = false.
+  Proof.
+    intros. split.
+    - apply bound_in_ge.
+    - cbn. destruct n.
+      + lia.
+      + intros.
+        rewrite leb_gt in H.
+        lia.
+  Qed.
+
+  Lemma bound_in_ind: forall ix n (P:Prop),
+      (ix >= n -> bound_in ix n = false -> P) ->
+      (ix < n -> bound_in ix n = true -> P) ->
+      P.
+  Proof.
+    introv.
+    rewrite <- bound_in_ge_iff.
+    rewrite <- bound_in_lt_iff.
+    introv Hge Hlt.
+    compare naturals ix and n; auto.
+    apply Hge; lia.
+  Qed.
+
+  Lemma bound_in_mono: forall ix n m,
+      m > n ->
+      bound_in ix n = true ->
+      bound_in ix m = true.
+  Proof.
+    introv Hlt Hbound.
+    rewrite <- bound_in_lt_iff in Hbound.
+    rewrite <- bound_in_lt_iff.
+    lia.
+  Qed.
+
+  Lemma bound_rev_mono: forall ix n m,
+      m < n ->
+      bound_in ix n = false ->
+      bound_in ix m = false.
+  Proof.
+    introv Hlt Hbound.
+    rewrite <- bound_in_ge_iff in Hbound.
+    rewrite <- bound_in_ge_iff.
+    lia.
+  Qed.
+
+  Lemma lift_lt: forall n depth ix,
+      ix < depth ->
+      lift n (depth, ix) = ix.
+  Proof.
+    intros. unfold lift.
+    rewrite bound_in_lt_iff in H.
+    now rewrite H.
+  Qed.
+
+  Lemma lift_ge: forall n depth ix,
+      ix >= depth ->
+      lift n (depth, ix) = ix + n.
+  Proof.
+    intros. unfold lift.
+    rewrite bound_in_ge_iff in H.
+    now rewrite H.
+  Qed.
+
+  Lemma lift_zero:
+    lift 0 = extract.
+  Proof.
+    ext [depth ix].
+    cbn.
+    destruct depth.
+    - lia.
+    - destruct (ix <=? depth); lia.
+  Qed.
+
+  Lemma lift_depth_zero: forall n ix,
+      lift n (0, ix) = ix + n.
+  Proof.
+    reflexivity.
+  Qed.
+
+End theory.
+
+Ltac bound_induction :=
+  match goal with
+  | |- context[bound_in ?ix ?n] =>
+      apply (bound_in_ind ix n);
+      let Hord := fresh "Hord" in
+      let Hbound := fresh "Hbound" in
+      introv Hord Hbound;
+      try rewrite Hbound in *;
+      try solve [lia | easy]
+  end.
 
 Section theory.
 
@@ -122,90 +298,80 @@ Section theory.
                         (unit := Monoid_unit_zero)
                         (op := Monoid_op_plus)}.
 
-  Lemma lift_zero:
-    lift 0 = extract.
+  Lemma lift_lift1: forall n m depth ix,
+      lift m (depth, lift n (depth, ix)) = lift (m + n) (depth, ix).
   Proof.
-    ext [depth ix].
-    cbn.
-    destruct depth.
-    - lia.
-    - destruct (ix <=? depth); lia.
+    intros. unfold lift.
+    - bound_induction.
+      + bound_induction.
+      + bound_induction.
+  Qed.
+
+  Lemma lift_lift2: forall (n m: nat),
+      lift m ⋆4 lift n = lift (m + n).
+  Proof.
+    intros. ext [depth ix].
+    unfold kc4, compose.
+    unfold_ops @Cobind_reader.
+    rewrite lift_lift1.
+    reflexivity.
   Qed.
 
   Lemma scoot_zero:
     scoot 0 = id.
   Proof.
-    unfold scoot.
-    ext σ ix.
-    cbn.
+    unfold scoot. ext σ ix. cbn.
     rewrite lift_zero.
     rewrite mapd_id.
     replace (ix - 0) with ix by lia.
     reflexivity.
   Qed.
 
-  Lemma lift1: forall (n m: nat),
-      lift m ⋆4 lift n = lift (m + n).
+  Lemma scoot_ren_zero:
+    scoot_ren 0 = id.
   Proof.
-    intros. ext p.
-    unfold kc4, compose.
-    unfold_ops @Cobind_reader.
-    cbn.
-    destruct p as [depth ix].
-    destruct depth.
-    - cbn. lia.
-    - cbn.
-      remember (ix <=? depth) as tmp.
-      destruct tmp.
-      rewrite <- Heqtmp.
-      reflexivity.
-      enough (ix + n <=? depth = false).
-      + rewrite H. lia.
-      + symmetry in Heqtmp.
-        rewrite Compare_dec.leb_iff_conv in *.
-        lia.
+    unfold scoot. ext σ ix. cbn.
+    replace (ix - 0) with ix by lia.
+    replace (σ ix + 0) with (σ ix) by lia.
+    reflexivity.
   Qed.
 
-  Lemma scoot1 : forall (n m: nat),
+  Lemma scoot_scoot : forall (n m: nat),
       scoot m ∘ scoot n = scoot (m + n).
   Proof.
-    intros.
-    ext σ. unfold compose.
-    ext ix.
-    unfold scoot, bound_in.
-    remember (ix <? m) as Hlt.
-    destruct Hlt; symmetry in HeqHlt.
-    - assert (Hlt2: ix <? m + n = true).
-      { rewrite PeanoNat.Nat.ltb_lt in *.
-        lia. }
-      rewrite Hlt2.
-      reflexivity.
-    -  rewrite PeanoNat.Nat.ltb_ge in HeqHlt.
-       assert ((ix - m <? n) = (ix <? m + n)).
-       { remember (ix <? m + n) as tmp.
-         destruct tmp; symmetry in Heqtmp.
-         - rewrite PeanoNat.Nat.ltb_lt in *.
-           lia.
-         - rewrite PeanoNat.Nat.ltb_ge in *.
-           lia.
-       }
-       rewrite H.
-       remember (ix <? m + n) as tmp.
-       destruct tmp.
-       { compose near (ix - m).
-         rewrite mapd_ret.
-         unfold_ops @Return_Writer.
-         unfold compose; cbn.
-         replace (ix - m + m) with ix by lia.
-         reflexivity.
-       }
-       { replace (ix - m - n) with (ix - (m + n)) by lia.
-         unfold compose.
-         compose near (σ (ix - (m + n))) on left.
-         rewrite mapd_mapd.
-         rewrite lift1.
-         reflexivity.
-       }
+    intros. ext σ ix.
+    unfold compose, scoot.
+    bound_induction.
+    - bound_induction.
+      + bound_induction.
+        { compose near (σ (ix - m - n)) on left.
+          rewrite mapd_mapd.
+          rewrite lift_lift2.
+          do 2 fequal. lia. }
+      + bound_induction.
+        { compose near (ix - m).
+          rewrite mapd_ret.
+          unfold compose; cbn.
+          fequal. lia. }
+    - bound_induction.
+  Qed.
+
+  Lemma scoot_ren_scoot_ren : forall (n m: nat),
+      scoot_ren m ∘ scoot_ren n = scoot_ren (m + n).
+  Proof.
+    intros. ext σ ix.
+    unfold compose, scoot_ren.
+    bound_induction.
+    - bound_induction.
+      + bound_induction.
+        rewrite lift_lift1.
+        do 2 rewrite lift_depth_zero.
+        do 2 fequal.
+        lia.
+      + bound_induction.
+        rewrite lift_depth_zero.
+        lia.
+    - bound_induction.
   Qed.
 
   Corollary scoot_S: forall (n: nat),
@@ -213,8 +379,77 @@ Section theory.
   Proof.
     intros.
     replace (S n) with (n + 1) by lia.
-    rewrite scoot1.
+    now rewrite scoot_scoot.
+  Qed.
+
+  Corollary scoot_ren_S: forall (n: nat),
+      scoot_ren (S n) = scoot_ren n ∘ scoot_ren 1.
+  Proof.
+    intros.
+    replace (S n) with (n + 1) by lia.
+    now rewrite scoot_ren_scoot_ren.
+  Qed.
+
+  Lemma iterate_scoot: forall n,
+      scoot n = iterate n (scoot 1).
+  Proof.
+    intros. induction n.
+    - rewrite scoot_zero. reflexivity.
+    - rewrite scoot_S.
+      rewrite IHn.
+      rewrite iterate_rw1.
+      reflexivity.
+  Qed.
+
+  Lemma scoot_ren_spec: forall ρ n,
+      ret ∘ (scoot_ren n ρ) = scoot n (ret ∘ ρ).
+  Proof.
+    intros.
+    ext m.
+    unfold compose; cbn.
+    unfold scoot, scoot_ren.
+    bound_induction.
+    compose near (ρ (m - n)).
+    rewrite (mapd_ret).
+    unfold compose.
     reflexivity.
+  Qed.
+
+  Lemma iterate_scoot_ren: forall n,
+      scoot_ren n = iterate n (scoot_ren 1).
+  Proof.
+    intros.
+    induction n.
+    - rewrite scoot_ren_zero.
+      reflexivity.
+    - rewrite scoot_ren_S.
+      rewrite IHn.
+      rewrite iterate_rw1.
+      reflexivity.
+  Qed.
+
+  Lemma rename_loc_preincr (ρ : nat -> nat) (n: nat):
+    rename_loc ρ ⦿ n =
+      rename_loc (scoot_ren n ρ).
+  Proof.
+    unfold rename_loc.
+    ext (depth, ix); cbn.
+    compose near ρ on right.
+    rewrite (scoot_ren_scoot_ren).
+    change (?n ● ?m) with (n + m).
+    fequal. lia.
+  Qed.
+
+  Lemma open_loc_preincr (σ : nat -> T nat) (n: nat):
+      open_loc σ ⦿ n =
+        open_loc (scoot n σ).
+  Proof.
+    unfold open_loc.
+    ext (depth, ix); cbn.
+    compose near σ on right.
+    rewrite (scoot_scoot).
+    change (?n ● ?m) with (n + m).
+    fequal. lia.
   Qed.
 
 End theory.
