Tealeaves/Backends/DB/Key.v
@@ -4,56 +4,19 @@ From Tealeaves Require Import
   Functors.Option.
 
 Open Scope nat_scope.
+
 Import
   List.ListNotations
   ContainerFunctor.Notations.
 
 Generalizable All Variables.
 
-Definition key :=
-  list atom.
-
-Fixpoint insert (k: key) (a: atom): key :=
-  match k with
-  | nil => [a]
-  | cons x rest =>
-      if a == x then k else x :: (insert rest a)
-                              (* (k ++ [a]) *)
-  end.
-
-Fixpoint get_index_rec (acc: nat) (a: atom) (k: key): option nat :=
-  match k with
-  | nil => None
-  | cons x rest =>
-      if a == x then Some acc else get_index_rec (S acc) a rest
-  end.
-
-Definition get_index: atom -> key -> option nat :=
-  get_index_rec 0.
-
-Fixpoint get_atom (k: key) (ix: nat): option atom :=
-  match k, ix with
-  | nil, _ => None
-  | cons a rest, 0 => Some a
-  | cons a rest, S ix => get_atom rest ix
-  end.
-
-(** ** Properties of <<insert>> *)
-(******************************************************************************)
-Lemma insert_cons_eq: forall a k x,
-    a = x ->
-    insert (a :: k) x = a :: k.
+Lemma nin_list_cons:
+  forall {A : Type} (a1 a2 : A) (xs : list A),
+    ~ a1 ∈ (a2 :: xs) <-> a1 <> a2 /\ ~ a1 ∈ xs.
 Proof.
-  intros. cbn.
-  destruct_eq_args x a.
-Qed.
-
-Lemma insert_cons_neq: forall a k x,
-    a <> x ->
-    insert (a :: k) x = a :: insert k x.
-Proof.
-  intros. cbn.
-  destruct_eq_args x a.
+  intros. rewrite in_list_cons.
+  intuition.
 Qed.
 
 Lemma map_some: forall `(f: A -> B) (x: option A)  y,
@@ -67,8 +30,287 @@ Proof.
   - inversion Heq.
 Qed.
 
+Definition key :=
+  list atom.
+
+Fixpoint unique (l: list atom): Prop :=
+  match l with
+  | nil => True
+  | cons a rest =>
+      ~ (a ∈ rest) /\ unique rest
+  end.
+
+Definition key_is_atom_in (k: key) (a: atom):
+  {a ∈ k} + {~ a ∈ k}.
+Proof.
+  induction k.
+  - right. inversion 1.
+  - pose (in_list_cons a a0 k).
+    destruct (a == a0).
+    + now (left; left).
+    + destruct IHk.
+      * now (left; right).
+      * right. rewrite i.
+        intros [contra|contra];
+          contradiction.
+Defined.
+
+Ltac compare_atoms :=
+    match goal with
+    | H: context[?a == ?a'] |- _ =>
+        destruct_eq_args a a'
+    | |- context[?a == ?a'] =>
+        destruct_eq_args a a'
+    end.
+
+Tactic Notation "compare" "atoms" := compare_atoms.
+
+Fixpoint key_insert_atom (k: key) (a: atom): key :=
+  match k with
+  | nil => [a]
+  | cons x rest =>
+      if a == x then k else
+        x :: key_insert_atom rest a
+  end.
+
+Lemma key_nin_insert: forall k a a',
+    a <> a' ->
+    ~ a ∈ k ->
+    ~ a ∈ key_insert_atom k a'.
+Proof.
+  introv Hneq Hnin. induction k.
+  - cbn. intros [H1|H2].
+    + now subst.
+    + assumption.
+  - rewrite nin_list_cons in Hnin.
+    destruct Hnin as [? Hnin].
+    specialize (IHk Hnin).
+    cbn. compare atoms.
+    + intros [contra|contra].
+      now subst. contradiction.
+    + intros [contra|contra].
+      now subst. contradiction.
+Qed.
+
+Lemma key_insert_unique (k: key) (a: atom):
+  unique k ->
+  unique (key_insert_atom k a).
+Proof.
+  intros.
+  induction k.
+  - cbn. easy.
+  - destruct H as [H1 H2].
+    specialize (IHk H2).
+    cbn. compare atoms.
+    cbn. split; auto.
+    apply key_nin_insert; auto.
+Qed.
+
+Fixpoint key_lookup_atom_rec (k: key) (acc: nat) (a: atom): option nat :=
+  match k with
+  | nil => None
+  | cons x rest =>
+      if a == x then Some acc else key_lookup_atom_rec rest (S acc) a
+  end.
+
+Definition key_lookup_atom_alt: key -> atom -> option nat :=
+  fun k => key_lookup_atom_rec k 0.
+
+Fixpoint key_lookup_atom (k: key) (a: atom): option nat :=
+  match k with
+  | [] => None
+  | x :: rest =>
+      if a == x
+      then Some 0
+      else map S (key_lookup_atom rest a)
+  end.
+
+Lemma key_lookup_atom_rec_spec (k: key) (a: atom) (n: nat):
+  key_lookup_atom_rec k n a = map (fun m => m + n) (key_lookup_atom k a).
+Proof.
+  generalize dependent n.
+  induction k; intro n.
+  - reflexivity.
+  - cbn. destruct (a == a0).
+    + reflexivity.
+    + rewrite (IHk (S n)).
+      compose near (key_lookup_atom k a) on right.
+      rewrite (fun_map_map).
+      fequal. ext m. cbn. lia.
+Qed.
+
+Lemma key_lookup_atom_spec (k: key) (a: atom):
+  key_lookup_atom_alt k a = key_lookup_atom k a.
+Proof.
+  unfold key_lookup_atom_alt.
+  rewrite key_lookup_atom_rec_spec.
+  replace (fun m => m + 0) with (@id nat).
+  now rewrite fun_map_id.
+  ext m. unfold id. lia.
+Qed.
+
+Fixpoint key_lookup_index (k: key) (ix: nat): option atom :=
+  match k, ix with
+  | nil, _ => None
+  | cons a rest, 0 => Some a
+  | cons a rest, S ix => key_lookup_index rest ix
+  end.
+
+Lemma key_lookup_not_in1:
+  forall (k:  key) (a: atom),
+    ~ a ∈ k -> key_lookup_atom k a = None.
+Proof.
+  intros. induction k.
+  - reflexivity.
+  - cbn.
+    rewrite nin_list_cons in H.
+    compare atoms.
+    rewrite IHk.
+    + reflexivity.
+    + intuition.
+Qed.
+
+Lemma key_lookup_not_in2:
+  forall (k:  key) (a: atom),
+    key_lookup_atom k a = None -> ~ a ∈ k.
+Proof.
+  intros k a hyp.
+  induction k.
+  - cbv. easy.
+  - rewrite nin_list_cons.
+    cbn in hyp.
+    compare atoms.
+    split.
+    + assumption.
+    + apply IHk.
+      destruct (key_lookup_atom k a).
+      * inversion hyp.
+      * reflexivity.
+Qed.
+
+Lemma key_lookup_not_in_iff:
+  forall (k:  key) (a: atom),
+    ~ a ∈ k <-> key_lookup_atom k a = None.
+Proof.
+  intros. split.
+  - apply key_lookup_not_in1.
+  - apply key_lookup_not_in2.
+Qed.
+
+Lemma key_lookup_ix:
+  forall (k:  key) (ix: nat) (a: atom),
+    key_lookup_index k ix = Some a -> a ∈ k.
+Proof.
+  introv Hin.
+  generalize dependent ix.
+  induction k; intros ix Hin.
+  - inversion Hin.
+  - destruct ix.
+    + cbn in *. inversion Hin. now left.
+    + cbn in Hin.
+      rewrite in_list_cons.
+      right. eauto.
+Qed.
+
+Lemma key_lookup_ix_length:
+  forall (k:  key) (ix: nat),
+    key_lookup_index k ix = None -> length k <= ix.
+Proof.
+  introv Hin.
+  generalize dependent ix.
+  induction k; intros ix Hin.
+  - cbn in *. lia.
+  - destruct ix.
+    + inversion Hin.
+    + cbn in *.
+      specialize (IHk _ Hin).
+      lia.
+Qed.
+
+Lemma key_lookup_in1:
+  forall (k:  key) (a: atom),
+    a ∈ k -> {n: nat | key_lookup_atom k a = Some n}.
+Proof.
+  introv Hin. induction k.
+  - inversion Hin.
+  - rewrite in_list_cons in Hin.
+    cbn. compare atoms.
+    + now (exists 0).
+    + assert (Hink: a ∈ k) by now inversion Hin.
+      destruct (IHk Hink) as [m Hm].
+      rewrite Hm.
+      now (exists (S m)).
+Qed.
+
+Lemma key_lookup_in2:
+  forall (k:  key) (a: atom) (n: nat),
+    key_lookup_atom k a = Some n -> a ∈ k.
+Proof.
+  intros k a.
+  induction k; intros n Heq.
+  - inversion Heq.
+  - rewrite in_list_cons.
+    cbn in Heq.
+    compare atoms.
+    + now left.
+    + right.
+      destruct (key_lookup_atom k a);
+        inversion Heq.
+      now eapply IHk.
+Qed.
+
+Lemma key_lookup:
+  forall (k: key) (a: atom),
+    {n: nat | key_lookup_atom k a = Some n /\ a ∈ k} +
+      {~ a ∈ k /\ key_lookup_atom k a = None}.
+Proof.
+  intros.
+  destruct (key_is_atom_in k a).
+  - left. destruct (key_lookup_in1 k a e) as [m Hm].
+    exists m. auto.
+  - right. split. assumption.
+    now apply key_lookup_not_in1.
+Defined.
+
+Ltac key_lookup k a :=
+  let n := fresh "n" in
+  let Hin := fresh "H_in" in
+  let Hnin := fresh "H_not_in" in
+  destruct (key_lookup k a) as
+    [[n [H_key_lookup Hin]] | [Hnin H_key_lookup]].
+
+Tactic Notation "lookup" constr(a) "in" "key" constr(k) := key_lookup k a.
+
+Goal forall k (a: atom), a ∈ k \/ ~ a ∈ k.
+Proof.
+  intros.
+  lookup a in key k.
+  - now left.
+  - now right.
+Qed.
+
+
+(** ** Properties of <<insert>> *)
+(******************************************************************************)
+Lemma insert_cons_eq: forall a k x,
+    a = x ->
+    key_insert_atom (a :: k) x = a :: k.
+Proof.
+  intros. cbn.
+  destruct_eq_args x a.
+Qed.
+
+Lemma insert_cons_neq: forall a k x,
+    a <> x ->
+    key_insert_atom (a :: k) x = a :: key_insert_atom k x.
+Proof.
+  intros. cbn.
+  destruct_eq_args x a.
+Qed.
+
 (** ** Properties of <<get_index>> *)
 (******************************************************************************)
+(*
 Lemma get_index_rec_S (acc: nat) (a: atom) (k: key):
   get_index_rec (S acc) a k = map S (get_index_rec acc a k).
 Proof.
@@ -113,9 +355,11 @@ Proof.
   apply (map_some (fun x => x + acc')).
   intros n m. lia.
 Qed.
+ *)
 
 (** *** Keys known to contain a particular element *)
 (******************************************************************************)
+(*
 Lemma get_index_rec_in (acc: nat) (x: atom) (k: key):
   x ∈ k -> exists ix, get_index_rec acc x k = Some ix.
 Proof.
@@ -143,7 +387,7 @@ Qed.
 
 Lemma get_index_rec_insert1 (acc: nat) (a: atom) (k: key) (x: atom):
   a = x ->
-  exists (m: nat), get_index_rec acc a (insert k x) = Some m.
+  exists (m: nat), get_index_rec acc a (key_insert_atom k x) = Some m.
 Proof.
   intro Heq.
   subst.
@@ -164,9 +408,13 @@ Proof.
   apply get_index_rec_insert1.
 Qed.
 
+
 Lemma get_atom_rw2: forall a k ix,
-    get_atom (a :: k) (S ix) = get_atom k ix.
+    key_lookup_atom_rec (a :: k) (S ix) =
+      key_lookup_atom_rec k ix.
 Proof.
+  intros.
+  cbn.
   reflexivity.
 Qed.
 
@@ -207,19 +455,32 @@ Proof.
   cbn.
   destruct_eq_args a x.
 Qed.
+*)
 
 (** ** Properties of <<get_atom>> *)
 (******************************************************************************)
-Lemma get_atom_0: forall a k ix,
+Lemma key_lookup_zero: forall a k ix,
     ix = 0 ->
-    get_atom (a :: k) ix = Some a.
+    key_lookup_index (a :: k) ix = Some a.
 Proof.
   intros. subst.
   reflexivity.
 Qed.
 
-Lemma get_index_cons: forall a x k ix,
-    get_index a (x :: k) = Some (S ix) ->
+Lemma key_lookup_hd: forall a a' k,
+    key_lookup_atom (a :: k) a' = Some 0 ->
+    a = a'.
+Proof.
+  introv Hlookup; cbn in *.
+  compare atoms.
+  lookup a' in key k;
+    rewrite H_key_lookup in Hlookup;
+    now inversion Hlookup.
+Qed.
+
+(*
+Lemma key_lookup_index_cons: forall a x k ix,
+    key_lookup_index a (x :: k) = Some (S ix) ->
     get_index a k = Some ix.
 Proof.
   introv HH.
@@ -232,43 +493,106 @@ Proof.
   lia.
   assumption.
 Qed.
+*)
 
-Lemma key_bijection1: forall a k ix,
-    get_index a k = Some ix ->
-    get_atom k ix = Some a.
+Lemma map_key_lookup_atom_S: forall k a ix,
+    map S (key_lookup_atom k a) = Some (S ix) ->
+    key_lookup_atom k a = Some ix.
 Proof.
   intros.
-  generalize dependent k.
-  induction ix.
-  - intro k. cbn. intro H.
-    destruct k.
-    + inversion H.
-    + apply get_index_Some_0 in H.
-      subst. reflexivity.
-  - intros k H.
-    destruct k.
-    + inversion H.
-    + rename a0 into x.
-      rewrite get_atom_rw2.
-      apply IHix.
-      eapply get_index_cons.
-      eassumption.
+  destruct (key_lookup_atom k a).
+  - cbn in H. inversion H. reflexivity.
+  - inversion H.
 Qed.
 
-Lemma key_bijection2: forall a k ix,
-    (* uniq k -> *)
-    get_atom k ix = Some a ->
-    get_index a k = Some ix.
+Lemma map_key_lookup_atom_Z: forall k a,
+    map S (key_lookup_atom_alt k a) = Some 0 -> False.
+Proof.
+  intros.
+  destruct (key_lookup_atom_alt k a).
+  - cbn in H. inversion H.
+  - inversion H.
+Qed.
+
+Lemma map_key_lookup_cons: forall a k a' ix,
+    key_lookup_atom (a :: k) a' = Some ix ->
+    (ix = 0 /\ a = a') \/
+      exists ix', ix = S ix' /\ key_lookup_atom k a' = Some ix'.
+Proof.
+  introv Hyp. cbn in Hyp.
+  compare atoms.
+  - left. inversion Hyp. intuition.
+  - right. destruct ix.
+    + false. destruct (key_lookup_atom k a').
+      * inversion Hyp.
+      * inversion Hyp.
+    + apply (map_key_lookup_atom_S k a' ix) in Hyp.
+      exists ix. split.  reflexivity. assumption.
+Qed.
+
+Lemma key_lookup_index_S: forall k ix a,
+    key_lookup_index k ix = Some a ->
+    forall a', key_lookup_index (a' :: k) (S ix) = Some a.
+Proof.
+  intros.
+  assumption.
+Qed.
+
+Lemma key_lookup_index_cons: forall a' a k ix,
+    key_lookup_index (a' :: k) ix = Some a ->
+    ix = 0 /\ a = a' \/
+      exists ix', ix = S ix' /\ key_lookup_index k ix' = Some a.
+Proof.
+  introv Hin. destruct ix.
+  - cbn in Hin. inversion Hin.
+    left. now split.
+  - cbn in Hin. right.
+    exists ix. split; auto.
+Qed.
+
+Lemma key_bijection1: forall a k ix,
+    key_lookup_atom k a = Some ix ->
+    key_lookup_index k ix = Some a.
 Proof.
   intros.
   generalize dependent ix.
-  induction k.
-  - cbn. inversion 1.
-  - introv hyp.
-    destruct ix.
-    + rewrite get_atom_0 in hyp; auto.
-      inversion hyp.
-      now apply get_index_Some_0.
-    + rewrite get_atom_rw2 in hyp.
-      apply IHk in hyp.
-Abort.
+  induction k; intros ix Hix.
+  - cbn in *. inversion Hix.
+  - apply map_key_lookup_cons in Hix.
+    destruct Hix as
+      [ [Hix1 Hix2] | [ix' [Heq Hlookup] ] ]; subst.
+    + subst. reflexivity.
+    + subst.
+      specialize (IHk _ Hlookup).
+      now apply key_lookup_index_S.
+Qed.
+
+Lemma key_bijection2: forall a k ix,
+    unique k ->
+    key_lookup_index k ix = Some a ->
+    key_lookup_atom k a = Some ix.
+Proof.
+  introv Huniq Hix.
+  generalize dependent ix.
+  induction k; intros ix Hix.
+  - cbn in Hix. inversion Hix.
+  - cbn.
+    apply key_lookup_index_cons in Hix.
+    destruct Hix as [[Hix_zero Heq] | [ix' [Heq Hrest]]].
+    + subst. compare atoms.
+    + destruct Huniq as [Hnin Huniq].
+      specialize (IHk Huniq).
+      compare atoms.
+      * false. apply key_lookup_ix in Hrest. contradiction.
+      * rewrite (IHk ix' Hrest).
+        reflexivity.
+Qed.
+
+Lemma key_bijection: forall a k ix,
+    unique k ->
+    key_lookup_index k ix = Some a <->
+      key_lookup_atom k a = Some ix.
+Proof.
+  intros.
+  split; auto using key_bijection1, key_bijection2.
+Qed.
