Tealeaves/Examples/STLC/Autosubst.v
@@ -1,0 +1,163 @@
+From Tealeaves Require Import
+  Backends.DB.DB
+  Theory.DecoratedTraversableMonad.
+
+From Autosubst Require Import
+  Autosubst.
+
+Export Kleisli.DecoratedTraversableMonad.Notations. (* ∈d *)
+Import Monoid.Notations. (* Ƶ and ● *)
+Import Misc.Subset.Notations. (* ∪ *)
+Export Applicative.Notations. (* <⋆> *)
+Export List.ListNotations. (* [] :: *)
+Export LN.AtomSet.Notations.
+Export LN.AssocList.Notations. (* one, ~ *)
+Export Product.Notations. (* × *)
+Export ContainerFunctor.Notations. (* ∈ *)
+Export DecoratedContainerFunctor.Notations. (* ∈d *)
+
+Set Implicit Arguments.
+
+(** ** Autosubst *)
+(******************************************************************************)
+Section Autosubst.
+
+  Inductive term (var : Type) : Type :=
+  | tvar (x : var)
+  | app (s t : term var)
+  | lam (s : {bind (term var)}).
+
+  #[export] Instance Ids_term : Ids (term var). derive. Defined.
+  #[export] Instance Rename_term : Rename (term var). derive. Defined.
+  #[export] Instance Subst_term : Subst (term var). derive. Defined.
+
+End Autosubst.
+
+Fixpoint binddt_term (G : Type -> Type) `{Map G} `{Pure G} `{Mult G}
+    {v1 v2 : Type} (f : nat * v1 -> G (term v2)) (t : term v1) : G (term v2) :=
+  match t with
+  | tvar v => f (0, v)
+  | lam body => pure (@lam _) <⋆> binddt_term (preincr f 1) body
+  | app t1 t2 => pure (@app v2) <⋆> binddt_term f t1 <⋆> binddt_term f t2
+  end.
+
+#[export] Instance Return_Term: Return term := tvar.
+#[export] Instance Binddt_Term: Binddt nat term term := @binddt_term.
+
+#[export] Instance Map_STLC: Map term
+  := Map_Binddt nat term term.
+#[export] Instance Mapd_STLC: Mapd nat term
+  := Mapd_Binddt nat term term.
+#[export] Instance Traverse_STLC: Traverse term
+  := Traverse_Binddt nat term term.
+#[export] Instance Mapdt_STLC: Mapdt nat term
+  := Mapdt_Binddt nat term term.
+#[export] Instance Bind_STLC: Bind term term
+  := Bind_Binddt nat term term.
+#[export] Instance Bindd_STLC: Bindd nat term term
+  := Bindd_Binddt nat term term.
+#[export] Instance Bindt_STLC: Bindt term term
+  := Bindt_Binddt nat term term.
+
+#[export] Instance DTMFull_Term:
+  DecoratedTraversableMonadFull nat term.
+Admitted.
+
+Implicit Types (ρ: nat -> nat) (σ: nat -> term nat).
+
+Ltac lia' :=
+  repeat
+  match goal with
+  | |- context[(?ix + 0)%nat] =>
+      replace (ix + 0)%nat with ix by lia
+  | |- context[(?ix - 0)%nat] =>
+      replace (ix - 0)%nat with ix by lia
+  | |- context[(?ix - ?m + ?m)%nat] => (* applies if ix > m in context *)
+      replace (ix - m + m)%nat with ix by lia
+  end;
+  try solve lia.
+
+Lemma upren_spec: forall ρ,
+    upren ρ = scoot_ren 1 ρ.
+Proof.
+  intros.
+  ext ix.
+  destruct ix.
+  - unfold scoot_ren. bound_induction.
+  - cbn.
+    replace (ix - 0) with ix by lia.
+    lia.
+Qed.
+
+Lemma Autosubst_rename_spec: forall (ρ: nat -> nat),
+    rename ρ =
+      DB.rename ρ.
+Proof.
+  intros. ext t.
+  generalize dependent ρ.
+  unfold DB.rename.
+  induction t; intro ρ.
+  - cbn; unfold compose.
+    unfold rename_loc.
+    now rewrite scoot_ren_zero.
+  - cbn.
+    rewrite IHt1.
+    rewrite IHt2.
+    reflexivity.
+  - cbn.
+    fequal.
+    change ((?f ∘ ?g) ⦿ ?n) with
+      (f ∘ (g ⦿ n)).
+    rewrite <- mapd_to_binddt.
+    rewrite rename_loc_preincr.
+    rewrite IHt.
+    rewrite upren_spec.
+    reflexivity.
+Qed.
+
+Import Coq.Init.Nat. (* Nat notations *)
+
+Lemma up_spec: forall (σ: nat -> term nat),
+    up σ = scoot 1 σ.
+Proof.
+  intros σ. ext n.
+  unfold up.
+  rewrite Autosubst_rename_spec.
+  unfold funcomp, scons, scoot, bound_in.
+  change (ids 0) with (ret 0).
+  remember (n <? 1) as b.
+  symmetry in Heqb.
+  destruct b.
+  - destruct n. easy. false.
+  - destruct n. easy.
+    cbn. lia'. unfold DB.rename.
+    fequal. ext [depth ix].
+    cbn. unfold scoot_ren.
+    + bound_induction.
+      cbn. lia'.
+      destruct depth. lia.
+      cbn in *.
+      rewrite Hbound. lia.
+      destruct depth.
+      lia. cbn in Hbound.
+      rewrite Hbound.
+      reflexivity.
+Qed.
+
+Lemma Tealeaves_Matches_Autosubst:
+  forall (t : term nat) (σ : nat -> term nat),
+    DB.open σ t = subst σ t.
+Proof.
+  intros. generalize dependent σ. induction t; intros σ.
+  - cbn. lia'.
+    rewrite DB.lift_zero.
+    rewrite dfun_mapd1.
+    reflexivity.
+  - cbn. fequal; eauto.
+  - cbn. fequal.
+    rewrite <- IHt.
+    unfold open.
+    rewrite open_loc_preincr.
+    rewrite up_spec.
+    reflexivity.
+Qed.
